proof/SimMemLiftInj.v
@@ -1,0 +1,69 @@
+Require Import CoqlibC.
+Require Import MemoryC.
+Require Import Values.
+Require Import Maps.
+Require Import Events.
+Require Import Globalenvs.
+Require Import AST.
+
+Require Import IntegersC LinkingC.
+Require Import SimSymb Skeleton Mod ModSem.
+Require Import SimMem SimMemLift.
+Require SimSymbId.
+Require Import Conventions1.
+Require Export SimMemInjC.
+
+Set Implicit Arguments.
+
+Global Program Instance lepriv_Transitive: RelationClasses.Transitive lepriv.
+Next Obligation.
+  ii. inv H; inv H0.
+  des; clarify.
+  econs; eauto with mem congruence.
+  + eapply inject_incr_trans; eauto.
+  + econs; eauto.
+    ii; des.
+    destruct (inj y b_src) eqn:T.
+    * destruct p.
+      exploit INCR0; eauto. i; clarify.
+      inv FROZEN.
+      hexploit NEW_IMPLIES_OUTSIDE; eauto.
+    * inv FROZEN0.
+      hexploit NEW_IMPLIES_OUTSIDE; eauto; []; i; des.
+      esplits; congruence.
+Qed.
+
+
+Global Program Instance SimMemInjLift : SimMemLift.class SimMemInjC.SimMemInj :=
+{
+  lift := lift';
+  unlift := unlift';
+}.
+Next Obligation.
+  rename H into VALID.
+  inv VALID. econs; ss; eauto; ii; des; ss; eauto.
+  - eapply Pos.compare_gt_iff in H. xomega.
+  - eapply Pos.compare_gt_iff in H. xomega.
+  - eapply Pos.compare_gt_iff in H. xomega.
+  - eapply Pos.compare_gt_iff in H. xomega.
+Qed.
+Next Obligation.
+  eapply unlift_spec; et.
+Qed.
+Next Obligation.
+  eapply unlift_wf; eauto.
+Qed.
+Next Obligation.
+  inv MWF.
+  destruct sm0; ss.
+  econs; ss; et.
+  - etrans; et.
+  - etrans; et.
+  - eapply frozen_refl.
+Qed.
+Next Obligation.
+  inv MWF. inv MLE. inv MLIFT.
+  (* destruct sm1; ss. *)
+  econs; ss; et; try congruence.
+  - eapply frozen_refl.
+Qed.
